Add till addAfter method

project.dfy
@@ -1,62 +1,289 @@
 module Collections {
+    
+    class Node {
+        var omLabel: int;
+        var omValue: int;
+
+        constructor (omLbl: int, omVal: int)
+        {
+            new;
+            omLabel := omLbl;
+            omValue := omVal;
+        }
+    }
 
     trait OMDataStructTrait
     {
-        ghost var omDsSeq: seq<int>;
+        var maxCapacity: int;
+        var omDS: array<Node?>;
+
+        ghost var omDsSeq: seq<Node?>;
 
         method addBefore(x: int, y: int)
             // Check y exists in DS
-            requires exists i :: 0 <= i < |omDsSeq| && omDsSeq[i] == y
+            requires exists i :: 0 <= i < |omDsSeq| && omDsSeq[i] != null && omDsSeq[i].omValue == y
             // Check x doesn't exist in DS
-            requires forall i :: 0 <= i < |omDsSeq| && omDsSeq[i] != x
+            requires forall i :: 0 <= i < |omDsSeq| && omDsSeq[i] != null && omDsSeq[i].omValue != x
             // Check x's position is less than y's position
-            ensures exists i,j :: 0 <= i < j < |omDsSeq| && omDsSeq[i] == x && omDsSeq[j] == y
+            ensures exists i,j :: 0 <= i < j < |omDsSeq| && (omDsSeq[i] != null && omDsSeq[i].omValue == x) && (omDsSeq[j] != null && omDsSeq[j].omValue == y)
+            modifies omDS, omDsSeq
 
         method addAfter(x: int, y: int)
             // Check y exists in DS
-            requires exists i :: 0 <= i < |omDsSeq| && omDsSeq[i] == y
+            requires exists i :: 0 <= i < |omDsSeq| && omDsSeq[i] != null && omDsSeq[i].omValue == y
             // Check x doesn't exist in DS
-            requires forall i :: 0 <= i < |omDsSeq| && omDsSeq[i] != x
+            requires forall i :: 0 <= i < |omDsSeq| && omDsSeq[i] != null && omDsSeq[i].omValue != x
             // Check x's position is greater than y's position
-            ensures exists i,j :: 0 <= i < j < |omDsSeq| && omDsSeq[i] == y && omDsSeq[j] == x
+            ensures exists i,j :: 0 <= i < j < |omDsSeq| && (omDsSeq[i] != null && omDsSeq[i].omValue == y) && (omDsSeq[j] != null && omDsSeq[j].omValue == x)
+            modifies omDS
 
         method add(x: int)
             // Check x doesn't exist in DS
-            requires forall i :: 0 <= i < |omDsSeq| && omDsSeq[i] != x
+            requires forall i :: 0 <= i < |omDsSeq| && omDsSeq[i] != null && omDsSeq[i].omValue != x
             // Check x exists random position in DS
-            ensures exists i :: 0 <= i < |omDsSeq| && omDsSeq[i] == x
+            ensures exists i :: 0 <= i < |omDsSeq| && omDsSeq[i] != null && omDsSeq[i].omValue == x
+            modifies omDS
 
-        method element(x: int) returns (exist: bool)
-            // At some position, if x exists then return true otherwise false
-            ensures exists i :: 0 <= i < |omDsSeq| && ((omDsSeq[i] == x && exist == true) || (omDsSeq[i] != x && exist == false))
+        // method element(x: int) returns (exist: bool)
+        //     // At some position, if x exists then return true otherwise false
+        //     ensures exists i :: 0 <= i < |omDsSeq| && ((omDsSeq[i] == x && exist == true) || (omDsSeq[i] != x && exist == false))
 
-        method before(x: int, y: int) returns (isBefore: bool)
-            // Checks x and y are different values
-            requires x != y
-            // Check x exists in DS
-            requires exists i :: 0 <= i < |omDsSeq| && omDsSeq[i] == x
+        // method before(x: int, y: int) returns (isBefore: bool)
+        //     // Checks x and y are different values
+        //     requires x != y
+        //     // Check x exists in DS
+        //     requires exists i :: 0 <= i < |omDsSeq| && omDsSeq[i] == x
+        //     // Check y exists in DS
+        //     requires exists j :: 0 <= j < |omDsSeq| && omDsSeq[j] == y
+        //     // If x's position is less than y's position then return true otherwise false
+        //     ensures exists i,j :: 0 <= i < j < |omDsSeq| && ((omDsSeq[i] == x && omDsSeq[j] == y && isBefore == true) || (omDsSeq[i] == y && omDsSeq[j] == x && isBefore == false))
+
+        // method append(x: int)
+        //     // Check x doesn't exist in DS
+        //     requires forall i :: 0 <= i < |omDsSeq| && omDsSeq[i] != x
+        //     // If DS size is 1 then x is at the start of DS or DS size is greater than 1 then x is at the end of the DS.
+        //     ensures ((|omDsSeq| == 1 && omDsSeq[0] == x) || (|omDsSeq| > 1 && omDsSeq[|omDsSeq|-1] == x))
+
+        // method prepend(x: int)
+        //     // Check x doesn't exist in DS
+        //     requires forall i :: 0 <= i < |omDsSeq| && omDsSeq[i] != x
+        //     // Check x is at the start of the DS always
+        //     ensures omDsSeq[0] == x
+
+        // method remove(x: int)
+        //     // Check x exists in DS
+        //     requires exists i :: 0 <= i < |omDsSeq| && omDsSeq[i] == x
+        //     // Check x doesn't exist in DS
+        //     ensures forall i :: 0 <= i < |omDsSeq| && omDsSeq[i] != x
+    }
+
+    class OMDataStruct extends OMDataStructTrait {
+        var randomNumber: int;
+
+        constructor (maxCap: int)
+            requires maxCap >= 0
+        {
+            new;
+            maxCapacity := maxCap;
+            randomNumber := 1;
+            // Temporary to test. Remove below.
+            maxCapacity := 16;
+            // TODO: Restrict max capacity to N
+            // TODO: label capacity - N^2
+            // Insert before 0 triggers relabeling. Thus, not covered in initial version.
+            // [0, 4, 8, 12] - labels
+            // [11, 46, 30, 4] - values
+            var node0 := new Node(0, 11);
+            var node1 := new Node(4, 46);
+            var node2 := new Node(8, 30);
+            var node3 := new Node(12, 4);
+
+            omDS := new Node?[maxCapacity];
+            omDS[0] := node0;
+            omDS[1] := node1;
+            omDS[2] := node2;
+            omDS[3] := node3;
+
+            omDsSeq := computerOmDsSeq(omDS, omDS.Length-1);
+        }
+
+        function computerOmDsSeq(omDS: array<Node?>, index: nat): seq<Node?>
+            requires 0 <= index < omDS.Length
+            reads omDS
+        {
+            if index == 0 then [omDS[0]] else computerOmDsSeq(omDS, index-1) + [omDS[index]]
+        }
+
+        // Will be used till a memory pointer manupulation way is found.
+        method findIndex(x: int) returns (index: int)
+            // Check y exists in the array
+            requires exists i :: 0 <= i < omDS.Length && omDS[i] != null && x == omDS[i].omValue
+            ensures 0 <= index < omDS.Length
+        {
+            index := 0;
+            while(index < omDS.Length)
+                // Swapping 2 invariants give an error
+                invariant 0 <= index <= omDS.Length
+                invariant forall i :: 0 <= i < index ==> omDS[i] == null || (omDS[i] != null && omDS[i].omValue != x)
+                decreases omDS.Length - index
+            {
+                if(omDS[index] != null && omDS[index].omValue == x) {
+                    break;
+                }
+
+                index := index + 1;
+            }
+        }
+
+        // This method of copying values and labels was added due to seq are immutable and arrays are fixed length.
+        // Method params are immutable.
+        method addValBeforeIndex(yIndex: int, x: int, xLabel: int)
+            requires exists i :: 0 <= i < omDS.Length && omDS[i] != null && i == yIndex
+            modifies omDS
+        {
+            var index: int := yIndex;
+
+            var yNode: Node := omDS[index];
+            omDS[index] := new Node(xLabel, x);
+            index := index + 1;
+
+            // Can't assert below. Should be a limitation of Dafny
+            // assert omDS[yIndex].omValue == x;
+
+            while(index < omDS.Length)
+                invariant yIndex+1 <= index <= omDS.Length
+                invariant forall i :: yIndex+1 <= i < index ==> omDS[i] != null
+                decreases omDS.Length - index
+            {
+                var yNodeNext := omDS[index];
+                omDS[index] := yNode;
+                if(yNodeNext == null) {
+                    break;
+                } else {
+                    yNode := yNodeNext;
+                }
+
+                index := index + 1;
+            }
+
+            // Can't assert below. Should be a limitation of Dafny
+            // assert exists i :: 0 <= i < omDS.Length ==> omDS[i] != null && omDS[i].omValue == x;
+        }
+
+        method addBefore(x: int, y: int)
             // Check y exists in DS
-            requires exists j :: 0 <= j < |omDsSeq| && omDsSeq[j] == y
-            // If x's position is less than y's position then return true otherwise false
-            ensures exists i,j :: 0 <= i < j < |omDsSeq| && ((omDsSeq[i] == x && omDsSeq[j] == y && isBefore == true) || (omDsSeq[i] == y && omDsSeq[j] == x && isBefore == false))
-
-        method append(x: int)
+            requires exists i :: 0 <= i < omDS.Length && omDS[i] != null && omDS[i].omValue == y
             // Check x doesn't exist in DS
-            requires forall i :: 0 <= i < |omDsSeq| && omDsSeq[i] != x
-            // If DS size is 1 then x is at the start of DS or DS size is greater than 1 then x is at the end of the DS.
-            ensures ((|omDsSeq| == 1 && omDsSeq[0] == x) || (|omDsSeq| > 1 && omDsSeq[|omDsSeq|-1] == x))
+            requires forall i :: 0 <= i < omDS.Length && omDS[i] != null && omDS[i].omValue != x
+            // Check x's position is less than y's position
+            modifies omDS
+        {
 
-        method prepend(x: int)
-            // Check x doesn't exist in DS
-            requires forall i :: 0 <= i < |omDsSeq| && omDsSeq[i] != x
-            // Check x is at the start of the DS always
-            ensures omDsSeq[0] == x
+            var yIndex: int := findIndex(y);
+            // yIndex = 0 should trigger relabelling. Thus, not covered in initial version.
+            if(yIndex > 0) {
+                var xLabel := (omDS[yIndex - 1].omLabel + omDS[yIndex].omLabel) / 2;
+                addValBeforeIndex(yIndex, x, xLabel);
+            }
 
-        method remove(x: int)
-            // Check x exists in DS
-            requires exists i :: 0 <= i < |omDsSeq| && omDsSeq[i] == x
-            // Check x doesn't exist in DS
-            ensures forall i :: 0 <= i < |omDsSeq| && omDsSeq[i] != x
+            // Can't assert below. Should be a limitation of Dafny
+            // assert exists i :: 0 <= i < omDS.Length ==> omDS[i] != null && y == omDS[i].omValue;
+            // assert exists i :: 0 <= i < omDS.Length && omDS[i] != null && x == omDS[i].omValue;
+        }
+
+        method addValAfterIndex(yIndex: int, x: int, xLabel: int)
+            requires exists i :: 0 <= i < omDS.Length && omDS[i] != null && i == yIndex
+            modifies omDS
+        {
+            var index: int := yIndex + 1;
+
+            // Otherwise needs relabelling or max capacity is reached.
+            if(index < omDS.Length) {
+
+                var yNodeNext: Node? := omDS[index];
+                omDS[index] := new Node(xLabel, x);
+                index := index + 1;
+
+                // Can't assert below. Should be a limitation of Dafny
+                // assert omDS[yIndex+1].omValue == x;
+
+                while(yNodeNext != null && index < omDS.Length)
+                    invariant yIndex+2 <= index <= omDS.Length
+                    invariant forall i :: yIndex+2 <= i < index ==> omDS[i] != null
+                    decreases omDS.Length - index
+                {
+                    var yNodeNextNext := omDS[index];
+                    omDS[index] := yNodeNext;
+                    if(yNodeNextNext == null) {
+                        break;
+                    } else {
+                        yNodeNext := yNodeNextNext;
+                    }
+
+                    index := index + 1;
+                }
+
+                // Can't assert below. Should be a limitation of Dafny
+                // assert exists i :: 0 <= i < omDS.Length ==> omDS[i] != null && omDS[i].omValue == x;
+            }
+        }
+
+        method addAfter(x: int, y: int)
+            // Check y exists in the array
+            requires exists i :: 0 <= i < omDS.Length && omDS[i] != null && y == omDS[i].omValue
+            // Check x doesn't exist in the array
+            requires forall i :: 0 <= i < omDS.Length && omDS[i] != null && x != omDS[i].omValue
+            modifies omDS
+        {
+            var yIndex: int := findIndex(y);
+            // yIndex = 0 should trigger relabelling. Thus, not covered in initial version.
+            var xLabel: int := 0;
+            if(yIndex == omDS.Length-1) {
+                xLabel := (omDS[yIndex].omLabel + (omDS.Length * omDS.Length)) / 2;
+            } else {
+                xLabel := (omDS[yIndex].omLabel + omDS[yIndex + 1].omLabel) / 2;
+            }
+            addValAfterIndex(yIndex, x, xLabel);
+        }
+
+        // method add(x: int)
+        //     // Check x doesn't exist in DS
+        //     requires forall i :: 0 <= i < omDS.Length && omDS[i] != null && omDS[i].omValue != x
+        //     modifies omDS
+        // {
+        //     var randomNumber: int := if omDS.Length == 0 then 0 else (randomNumber % omDS.Length) - 1;
+        //     var yIndex: int := randomNumber;
+        //     var xLabel: int := 0;
+        //     if(yIndex == omDS.Length-1) {
+        //         xLabel := (omDS[yIndex].omLabel + (omDS.Length * omDS.Length)) / 2;
+        //     } else {
+        //         xLabel := (omDS[yIndex].omLabel + omDS[yIndex + 1].omLabel) / 2;
+        //     }
+        //     randomNumber := randomNumber + 1;
+            
+        //     addValBeforeIndex(yIndex, x, xLabel);
+        // }
+
+        // method element(x: int) returns (exist: bool)
+        // {
+
+        // }
+
+        // method before(x: int, y: int) returns (isBefore: bool)
+        // {
+            
+        // }
     }
     
+}
+
+module Runner {
+    // import c = Collections
+
+    // method main()
+    // {
+    //     var omDataStruct := new c.OMDataStruct(16);
+
+    //     omDataStruct.addBefore(8, 30);
+    // }
 }
